cp; opening

examples/dsls/core/Refl.Typing.fsti
@@ -16,10 +16,6 @@ let lookup_bvar_extend_env (g:env) (x y:var) (ty:term)
     [SMTPat (lookup_bvar (extend_env g x ty) y)]
   = admit()
 
-//replace BV 0 in t with v
-val open_with (t:term) (v:term) : term
-val open_term (t:term) (v:var) : term
-val close_term (t:term) (v:var) : term
 let as_binder (x:var) (ty:term)
   : binder 
   = pack_binder
@@ -31,14 +27,6 @@ let as_binder (x:var) (ty:term)
 
 let bv_index (x:bv) : int = (inspect_bv x).bv_index
 
-let make_bv (n:nat) (t:term) = { bv_ppname = "_"; bv_index = n; bv_sort = t}
-
-let bv_as_binder bv = pack_binder bv Q_Explicit []
-
-let bv_index_of_make_bv (n:nat) (t:term)
-  : Lemma (ensures bv_index (pack_bv (make_bv n t)) == n)
-          [SMTPat (bv_index (pack_bv (make_bv n t)))]
-  = admit()
 
 let binder_sort (b:binder) =
   let bv, _ = inspect_binder b in 
@@ -48,6 +36,213 @@ let binder_sort_lemma (x:var) (ty:term)
   : Lemma (binder_sort (as_binder x ty) == ty)
           [SMTPat (binder_sort (as_binder x ty))]
   = admit()          
+
+//replace BV 0 in t with v
+val open_ctx_uvar_and_subst (c:ctx_uvar_and_subst) (v:term) (i:nat) 
+  : ctx_uvar_and_subst
+
+noeq
+type open_or_close =
+  | Open of term
+  | Close of var
+  
+let rec open_term' (t:term) (v:term) (i:nat)
+  : GTot term (decreases t)
+  = match inspect_ln t with
+    | Tv_Var _
+    | Tv_FVar _
+    | Tv_Type _
+    | Tv_Const _
+    | Tv_Unknown -> t
+    | Tv_BVar j -> 
+      if i=bv_index j 
+      then v
+      else t
+      
+    | Tv_App hd argv ->
+      pack_ln (Tv_App (open_term' hd v i)
+                      (open_term' (fst argv) v i, snd argv))
+
+    | Tv_Abs b body -> 
+      let b' = open_binder' b v i in
+      pack_ln (Tv_Abs b' (open_term' body v (i + 1)))
+
+    | Tv_Arrow b c ->
+      let b' = open_binder' b v i in
+      pack_ln (Tv_Arrow b' (open_comp' c v (i + 1)))      
+
+    | Tv_Refine bv f ->
+      assume (bv << t); //bug in the definition of R.smaller
+      let bv' = open_bv' bv v i in
+      pack_ln (Tv_Refine bv' (open_term' f v (i + 1)))
+
+    | Tv_Uvar j c ->
+      pack_ln (Tv_Uvar j (open_ctx_uvar_and_subst c v i))
+      
+    | Tv_Let recf attrs bv def body ->
+      assume (attrs << t); //bug in defn of R.smaller
+      pack_ln (Tv_Let recf 
+                      (open_terms' attrs v i)
+                      (open_bv' bv v i)
+                      (if recf 
+                       then open_term' def v (i + 1)
+                       else open_term' def v i)
+                      (open_term' body v (i + 1)))
+
+    | Tv_Match scr ret brs ->
+      assume (brs << t);
+      pack_ln (Tv_Match (open_term' scr v i)
+                        (match ret with
+                         | None -> None
+                         | Some m -> Some (open_match_returns' m v i))
+                        (open_branches' brs v i))
+      
+    | Tv_AscribedT e t tac b ->
+      pack_ln (Tv_AscribedT (open_term' e v i)
+                            (open_term' t v i)
+                            (match tac with
+                             | None -> None
+                             | Some tac -> Some (open_term' tac v i))
+                             b)
+
+    | Tv_AscribedC e c tac b ->
+      pack_ln (Tv_AscribedC (open_term' e v i)
+                            (open_comp' c v i)
+                            (match tac with
+                             | None -> None
+                             | Some tac -> Some (open_term' tac v i))
+                             b)
+
+and open_bv' (b:bv) (v:term) (i:nat)
+  : GTot bv (decreases b)
+  = let bv = inspect_bv b in
+    assume (bv << b);
+    pack_bv ({bv with bv_sort = open_term' bv.bv_sort v i})
+
+and open_binder' (b:binder) (v:term) (i:nat)
+  : GTot binder (decreases b)
+  = let bndr  = inspect_binder b in
+    assume (bndr << b);
+    let bv, (q, attrs) = bndr in
+    pack_binder (open_bv' bv v i) 
+                q
+                (open_terms' attrs v i)
+
+and open_comp' (c:comp) (v:term) (i:nat)
+  : GTot comp (decreases c)
+  = match inspect_comp c with
+    | C_Total t decr ->
+      pack_comp (C_Total (open_term' t v i)
+                         (open_terms' decr v i))
+
+    | C_GTotal t decr ->
+      pack_comp (C_GTotal (open_term' t v i)
+                          (open_terms' decr v i))
+
+    | C_Lemma pre post pats ->
+      pack_comp (C_Lemma (open_term' pre v i)
+                         (open_term' post v i)
+                         (open_term' pats v i))
+
+    | C_Eff us eff_name res args ->
+      assume (args << c);
+      pack_comp (C_Eff us eff_name
+                       (open_term' res v i)
+                       (open_args' args v i))
+
+and open_terms' (ts:list term) (v:term) (i:nat)
+  : GTot (list term) (decreases ts)
+  = match ts with
+    | [] -> []
+    | t::ts -> open_term' t v i :: open_terms' ts v i
+
+and open_args' (ts:list argv) (v:term) (i:nat)
+  : GTot (list argv) (decreases ts)
+  = match ts with
+    | [] -> []
+    | (t,q)::ts -> (open_term' t v i,q) :: open_args' ts v i
+
+and open_patterns' (ps:list (pattern & bool)) (v:term) (i:nat) 
+  : GTot (list (pattern & bool) & nat)
+         (decreases ps)
+  = match ps with
+    | [] -> ps, 0
+    | (p, b)::ps ->
+      let (p, n) = open_pattern' p v i in
+      let (ps, m) = open_patterns' ps v (i + n) in
+      (p,b)::ps, n + m
+
+and open_pattern' (p:pattern) (v:term) (i:nat) 
+  : GTot (pattern & nat)
+         (decreases p)
+  = match p with
+    | Pat_Constant _ -> p,0
+
+    | Pat_Cons fv pats -> 
+      let pats, n = open_patterns' pats v i in
+      Pat_Cons fv pats, n
+      
+    | Pat_Var bv ->
+      Pat_Var (open_bv' bv v i), 1
+
+    | Pat_Wild bv ->
+      Pat_Wild (open_bv' bv v i), 1
+
+    | Pat_Dot_Term bv t -> //CHECK!
+      Pat_Dot_Term (open_bv' bv v i) (open_term' t v i), 0
+
+    
+and open_branch' (br:branch) (v:term) (i:nat)
+  : GTot branch (decreases br)
+  = let p, t = br in
+    let p, j = open_pattern' p v i in
+    let t = open_term' t v (i + j) in
+    p, t
+  
+and open_branches' (brs:list branch) (v:term) (i:nat)
+  : GTot (list branch) (decreases brs)
+  = match brs with
+    | [] -> []
+    | br::brs -> open_branch' br v i :: open_branches' brs v i
+  
+and open_match_returns' (m:match_returns_ascription) (v:term) (i:nat)
+  : GTot match_returns_ascription (decreases m)
+  = let b, (ret, as_, eq) = m in
+    let b = open_binder' b v i in
+    let ret =
+      match ret with
+      | Inl t -> Inl (open_term' t v (i + 1))
+      | Inr c -> Inr (open_comp' c v (i + 1))
+    in
+    let as_ =
+      match as_ with
+      | None -> None
+      | Some t -> Some (open_term' t v (i + 1))
+    in
+    b, (ret, as_, eq)
+
+
+val open_term_with (t:term) (v:term) : t':term { t' == open_term' t v 0 }
+let make_bv (n:nat) (t:term) = { bv_ppname = "_"; bv_index = n; bv_sort = t}
+let var_as_term (v:var) = pack_ln (Tv_Var (pack_bv (make_bv v (pack_ln Tv_Unknown))))
+
+val open_term (t:term) (v:var) : t':term { t' == open_term' t (var_as_term v) 0 }
+val close_term (t:term) (v:var) : term
+
+
+
+
+
+
+
+
+
+let bv_as_binder bv = pack_binder bv Q_Explicit []
+
+let bv_index_of_make_bv (n:nat) (t:term)
+  : Lemma (ensures bv_index (pack_bv (make_bv n t)) == n)
+          [SMTPat (bv_index (pack_bv (make_bv n t)))]
+  = admit()
 
 let constant_as_term (v:vconst) = pack_ln (Tv_Const v)
 let unit_exp = constant_as_term C_Unit
@@ -167,4 +362,6 @@ and sub_typing : env -> term -> term -> Type0 =
       t:term ->
       sub_typing g t t
 
+  | ST_RefineLeft:
+  
 and branches_typing : env -> term -> term -> list branch -> term -> Type0 =
